merging closed refinement manually

simulations/hmodsim/HPSim.v
@@ -34,7 +34,7 @@ Section HPSIM.
   Definition dummy_term (with_dummy: bool) : itree hmodE unit :=
     if with_dummy then trigger (Guarantee True) else Ret tt.
   
-  Variant _hpsim' {with_dummy: bool}
+  Variant _hpsim' {with_dummy: bool} (is_closed: bool)
     (hpsimc: forall R (RR: nat -> alist key Any.t * R -> alist key Any.t * R -> iProp), bool -> bool -> nat -> alist key Any.t * itree hmodE R -> alist key Any.t * itree hmodE R -> Σ -> Prop)
     {R} {RR: nat -> alist key Any.t * R -> alist key Any.t * R -> iProp} (hpsimi: bool -> bool -> nat -> alist key Any.t * itree hmodE R -> alist key Any.t * itree hmodE R -> Σ -> Prop)
     : bool -> bool -> nat -> alist key Any.t * itree hmodE R -> alist key Any.t * itree hmodE R -> Σ -> Prop :=
@@ -45,7 +45,7 @@ Section HPSIM.
       v_src v_tgt
       (RET: Own fmr ⊢ #=> RR nths (st_src,v_src) (st_tgt,v_tgt))
     :
-    _hpsim' hpsimc hpsimi ps pt nths (st_src, Ret v_src) (st_tgt, Ret v_tgt) fmr
+    _hpsim' is_closed hpsimc hpsimi ps pt nths (st_src, Ret v_src) (st_tgt, Ret v_tgt) fmr
 
   | hpsim_call
       (HPSIM_CALL: True)
@@ -58,7 +58,7 @@ Section HPSIM.
                  (INV: Own fmr0 ⊢ #=> (Ist nths0 st_src0 st_tgt0 ∗ FR)),
           hpsimi true true nths0 (st_src0, k_src vret) (st_tgt0, k_tgt vret) fmr0)				
     :
-    _hpsim' hpsimc hpsimi ps pt nths (st_src, trigger (Call fn varg) >>= k_src) (st_tgt, trigger (Call fn varg) >>= k_tgt) fmr
+    _hpsim' is_closed hpsimc hpsimi ps pt nths (st_src, trigger (Call fn varg) >>= k_src) (st_tgt, trigger (Call fn varg) >>= k_tgt) fmr
 
   | hpsim_io
       (HPSIM_IO: True)
@@ -67,7 +67,7 @@ Section HPSIM.
       (K: forall (vret: O), 
     hpsimi true true nths (st_src, k_src vret) (st_tgt, k_tgt vret) fmr)
     :
-    _hpsim' hpsimc hpsimi ps pt nths (st_src, trigger (IO fn varg) >>= k_src) (st_tgt, trigger (IO fn varg) >>= k_tgt) fmr
+    _hpsim' is_closed hpsimc hpsimi ps pt nths (st_src, trigger (IO fn varg) >>= k_src) (st_tgt, trigger (IO fn varg) >>= k_tgt) fmr
 
   | hpsim_inline_src
       (HPSIM_INLINE_SRC: True)
@@ -76,7 +76,7 @@ Section HPSIM.
       (FUN: alist_find fn fl_src = Some f)
       (K: hpsimi true pt nths (st_src, f varg >>= (fun x => dummy_term with_dummy;;; tau;; Ret x) >>= k_src) (st_tgt, i_tgt) fmr)
     :
-    _hpsim' hpsimc hpsimi ps pt nths (st_src, trigger (Call fn varg) >>= k_src) (st_tgt, i_tgt) fmr
+    _hpsim' is_closed hpsimc hpsimi ps pt nths (st_src, trigger (Call fn varg) >>= k_src) (st_tgt, i_tgt) fmr
 
   | hpsim_inline_tgt
       (HPSIM_INLINE_TGT: True)
@@ -85,7 +85,7 @@ Section HPSIM.
       (FUN: alist_find fn fl_tgt = Some f)
       (K: hpsimi ps true nths (st_src, i_src) (st_tgt, f varg >>= (fun x => dummy_term with_dummy;;; tau;; Ret x) >>= k_tgt) fmr)
     :
-    _hpsim' hpsimc hpsimi ps pt nths (st_src, i_src) (st_tgt, trigger (Call fn varg) >>= k_tgt) fmr
+    _hpsim' is_closed hpsimc hpsimi ps pt nths (st_src, i_src) (st_tgt, trigger (Call fn varg) >>= k_tgt) fmr
 
   | hpsim_tau_src
       (HPSIM_TAU_SRC: True)
@@ -93,7 +93,7 @@ Section HPSIM.
       i_src i_tgt
       (K: hpsimi true pt nths (st_src, i_src) (st_tgt, i_tgt) fmr)
     :
-    _hpsim' hpsimc hpsimi ps pt nths (st_src, tau;; i_src) (st_tgt, i_tgt) fmr
+    _hpsim' is_closed hpsimc hpsimi ps pt nths (st_src, tau;; i_src) (st_tgt, i_tgt) fmr
 
   | hpsim_tau_tgt
       (HPSIM_TAU_TGT: True)
@@ -101,7 +101,7 @@ Section HPSIM.
       i_src i_tgt
       (K: hpsimi ps true nths (st_src, i_src) (st_tgt, i_tgt) fmr)
     :
-    _hpsim' hpsimc hpsimi ps pt nths (st_src, i_src) (st_tgt, tau;; i_tgt) fmr
+    _hpsim' is_closed hpsimc hpsimi ps pt nths (st_src, i_src) (st_tgt, tau;; i_tgt) fmr
 
   | hpsim_take_src
       (HPSIM_TAKE_SRC: True)
@@ -109,7 +109,7 @@ Section HPSIM.
       X k_src i_tgt
       (K: forall (x: X), hpsimi true pt nths (st_src, k_src x) (st_tgt, i_tgt) fmr)
     :
-    _hpsim' hpsimc hpsimi ps pt nths (st_src, trigger (Take X) >>= k_src) (st_tgt, i_tgt) fmr
+    _hpsim' is_closed hpsimc hpsimi ps pt nths (st_src, trigger (Take X) >>= k_src) (st_tgt, i_tgt) fmr
             
   | hpsim_choose_tgt
       (HPSIM_CHOOSE_TGT: True)
@@ -117,7 +117,7 @@ Section HPSIM.
       X i_src k_tgt
       (K: forall (x: X), hpsimi ps true nths (st_src, i_src) (st_tgt, k_tgt x) fmr)
     :
-    _hpsim' hpsimc hpsimi ps pt nths (st_src, i_src) (st_tgt, trigger (Choose X) >>= k_tgt) fmr
+    _hpsim' is_closed hpsimc hpsimi ps pt nths (st_src, i_src) (st_tgt, trigger (Choose X) >>= k_tgt) fmr
 
   | hpsim_choose_src
       (HPSIM_CHOOSE_SRC: True)
@@ -125,7 +125,7 @@ Section HPSIM.
       X x k_src i_tgt
       (K: hpsimi true pt nths (st_src, k_src x) (st_tgt, i_tgt) fmr)
     :
-    _hpsim' hpsimc hpsimi ps pt nths (st_src, trigger (Choose X) >>= k_src) (st_tgt, i_tgt) fmr
+    _hpsim' is_closed hpsimc hpsimi ps pt nths (st_src, trigger (Choose X) >>= k_src) (st_tgt, i_tgt) fmr
 
   | hpsim_take_tgt
       (HPSIM_TAKE_TGT: True)
@@ -133,7 +133,7 @@ Section HPSIM.
       X x i_src k_tgt
       (K: hpsimi ps true nths (st_src, i_src) (st_tgt, k_tgt x) fmr)
     :
-    _hpsim' hpsimc hpsimi ps pt nths (st_src, i_src) (st_tgt, trigger (Take X) >>= k_tgt) fmr
+    _hpsim' is_closed hpsimc hpsimi ps pt nths (st_src, i_src) (st_tgt, trigger (Take X) >>= k_tgt) fmr
 
   | hpsim_sput_src
       (HPSIM_SPUT_SRC: True)
@@ -143,7 +143,7 @@ Section HPSIM.
       (run: st_src0 = alist_upd k v st_src)
       (K: hpsimi true pt nths (st_src0, k_src tt) (st_tgt, i_tgt) fmr)
     :
-    _hpsim' hpsimc hpsimi ps pt nths (st_src, trigger (SPut k v) >>= k_src) (st_tgt, i_tgt) fmr
+    _hpsim' is_closed hpsimc hpsimi ps pt nths (st_src, trigger (SPut k v) >>= k_src) (st_tgt, i_tgt) fmr
 
   | hpsim_sput_tgt
       (HPSIM_SPUT_SRC: True)
@@ -153,7 +153,7 @@ Section HPSIM.
       (run: st_tgt0 = alist_upd k v st_tgt)
       (K: hpsimi ps true nths (st_src, i_src) (st_tgt0, k_tgt tt) fmr)
     :
-    _hpsim' hpsimc hpsimi ps pt nths (st_src, i_src) (st_tgt, trigger (SPut k v) >>= k_tgt) fmr
+    _hpsim' is_closed hpsimc hpsimi ps pt nths (st_src, i_src) (st_tgt, trigger (SPut k v) >>= k_tgt) fmr
 
   | hpsim_sget_src
       (HPSIM_SPUT_SRC: True)
@@ -163,7 +163,7 @@ Section HPSIM.
       (run: v = or_else (alist_find k st_src) tt↑)
       (K: hpsimi true pt nths (st_src, k_src v) (st_tgt, i_tgt) fmr)
     :
-    _hpsim' hpsimc hpsimi ps pt nths (st_src, trigger (SGet k) >>= k_src) (st_tgt, i_tgt) fmr
+    _hpsim' is_closed hpsimc hpsimi ps pt nths (st_src, trigger (SGet k) >>= k_src) (st_tgt, i_tgt) fmr
  
   | hpsim_sget_tgt
       (HPSIM_SPUT_SRC: True)
@@ -173,7 +173,7 @@ Section HPSIM.
       (run: v = or_else (alist_find k st_tgt) tt↑)
       (K: hpsimi ps true nths (st_src, i_src) (st_tgt, k_tgt v) fmr)
     :
-    _hpsim' hpsimc hpsimi ps pt nths (st_src, i_src) (st_tgt, trigger (SGet k) >>= k_tgt) fmr
+    _hpsim' is_closed hpsimc hpsimi ps pt nths (st_src, i_src) (st_tgt, trigger (SGet k) >>= k_tgt) fmr
  
   | hpsim_assume_src
       (HPSIM_ASSUME_SRC: True)
@@ -183,7 +183,7 @@ Section HPSIM.
       (K: forall fmr0 (NEW: Own fmr0 ⊢ #=> (iP ∗ FMR)),
           hpsimi true pt nths (st_src, k_src tt) (st_tgt, i_tgt) fmr0)
     :
-    _hpsim' hpsimc hpsimi ps pt nths (st_src, trigger (Assume iP) >>= k_src) (st_tgt, i_tgt) fmr
+    _hpsim' is_closed hpsimc hpsimi ps pt nths (st_src, trigger (Assume iP) >>= k_src) (st_tgt, i_tgt) fmr
 
   | hpsim_guarantee_tgt
       (HPSIM_GUARANTEE_TGT: True)
@@ -193,7 +193,7 @@ Section HPSIM.
       (K: forall fmr0 (NEW: Own fmr0 ⊢ #=> (iP ∗ FMR)),
           hpsimi ps true nths (st_src, i_src) (st_tgt, k_tgt tt) fmr0)
     :
-    _hpsim' hpsimc hpsimi ps pt nths (st_src, i_src) (st_tgt, trigger (Guarantee iP) >>= k_tgt) fmr
+    _hpsim' is_closed hpsimc hpsimi ps pt nths (st_src, i_src) (st_tgt, trigger (Guarantee iP) >>= k_tgt) fmr
             
   | hpsim_guarantee_src
       (HPSIM_GUARANTEE_SRC: True)
@@ -203,7 +203,7 @@ Section HPSIM.
       (K: forall fmr0 (NEW: Own fmr0 ⊢ #=> FMR),
           hpsimi true pt nths (st_src, k_src tt) (st_tgt, i_tgt) fmr0)
     :
-    _hpsim' hpsimc hpsimi ps pt nths (st_src, trigger (Guarantee iP) >>= k_src) (st_tgt, i_tgt) fmr
+    _hpsim' is_closed hpsimc hpsimi ps pt nths (st_src, trigger (Guarantee iP) >>= k_src) (st_tgt, i_tgt) fmr
 
   | hpsim_assume_tgt
       (HPSIM_ASSUME_TGT: True)
@@ -213,7 +213,7 @@ Section HPSIM.
       (K: forall fmr0 (NEW: Own fmr0 ⊢ #=> FMR),
           hpsimi ps true nths (st_src, i_src) (st_tgt, k_tgt tt) fmr0)
     :
-    _hpsim' hpsimc hpsimi ps pt nths (st_src, i_src) (st_tgt, trigger (Assume iP) >>= k_tgt) fmr
+    _hpsim' is_closed hpsimc hpsimi ps pt nths (st_src, i_src) (st_tgt, trigger (Assume iP) >>= k_tgt) fmr
 
   | hpsim_spawn
       (HPSIM_SPAWN: True)
@@ -221,7 +221,7 @@ Section HPSIM.
       fn arg k_src k_tgt
       (K: hpsimi true true (S nths) (st_src, k_src nths) (st_tgt, k_tgt nths) fmr)
     :
-    _hpsim' hpsimc hpsimi ps pt nths (st_src, trigger (Spawn fn arg) >>= k_src) (st_tgt, trigger (Spawn fn arg) >>= k_tgt) fmr
+    _hpsim' is_closed hpsimc hpsimi ps pt nths (st_src, trigger (Spawn fn arg) >>= k_src) (st_tgt, trigger (Spawn fn arg) >>= k_tgt) fmr
 
   | hpsim_yield
       (HPSIM_YIELD: True)
@@ -234,7 +234,7 @@ Section HPSIM.
                  (INV: Own fmr0 ⊢ #=> (Ist nths0 st_src0 st_tgt0 ∗ FR)),
           hpsimi true true nths0 (st_src0, k_src tt) (st_tgt0, k_tgt tt) fmr0)				
     :
-    _hpsim' hpsimc hpsimi ps pt nths (st_src, trigger (Yield tid) >>= k_src) (st_tgt, trigger (Yield tid) >>= k_tgt) fmr
+    _hpsim' is_closed hpsimc hpsimi ps pt nths (st_src, trigger (Yield tid) >>= k_src) (st_tgt, trigger (Yield tid) >>= k_tgt) fmr
         
   | hpsim_tid_src
       (HPSIM_TID_SRC: True)
@@ -242,7 +242,7 @@ Section HPSIM.
       k_src i_tgt
       (K: hpsimi true pt nths (st_src, k_src my_tid) (st_tgt, i_tgt) fmr)
     :
-    _hpsim' hpsimc hpsimi ps pt nths (st_src, trigger Tid >>= k_src) (st_tgt, i_tgt) fmr
+    _hpsim' is_closed hpsimc hpsimi ps pt nths (st_src, trigger Tid >>= k_src) (st_tgt, i_tgt) fmr
 
   | hpsim_tid_tgt
       (HPSIM_TID_TGT: True)
@@ -250,30 +250,41 @@ Section HPSIM.
       i_src k_tgt
       (K: hpsimi ps true nths (st_src, i_src) (st_tgt, k_tgt my_tid) fmr)
     :
-    _hpsim' hpsimc hpsimi ps pt nths (st_src, i_src) (st_tgt, trigger Tid >>= k_tgt) fmr
+    _hpsim' is_closed hpsimc hpsimi ps pt nths (st_src, i_src) (st_tgt, trigger Tid >>= k_tgt) fmr
+
+  | hpsim_call_none
+      (HPSIM_CALL_NONE: True)
+      ps pt nths st_src st_tgt fmr
+      fn varg i_src k_tgt
+      (CLOSED: is_closed = true)
+      (FUN: alist_find fn fl_tgt = None)
+      (K: hpsimi ps true nths (st_src, i_src) (st_tgt, triggerNB >>= k_tgt) fmr)
+    :
+    _hpsim' is_closed hpsimc hpsimi ps pt nths (st_src, i_src) (st_tgt, trigger (Call fn varg) >>= k_tgt) fmr
 
   | hpsim_progress
       (HPSIM_PROGRESS: True)
       nths sti_src sti_tgt fmr
       (SIM: hpsimc R RR false false nths sti_src sti_tgt fmr)
     :
-    _hpsim' hpsimc hpsimi true true nths sti_src sti_tgt fmr
+    _hpsim' is_closed hpsimc hpsimi true true nths sti_src sti_tgt fmr
   .
-  Arguments _hpsim' {with_dummy} hpsimc {R} RR hpsimi.
+  Arguments _hpsim' {with_dummy} is_closed hpsimc {R} RR hpsimi.
 
-  Inductive _hpsim {with_dummy} hpsim R RR ps pt nths sti_src sti_tgt fmr : Prop
+  Inductive _hpsim {with_dummy} is_closed hpsim R RR ps pt nths sti_src sti_tgt fmr : Prop
     :=
-  | hpsim_intro (IN: hsupd (@_hpsim' with_dummy hpsim R RR (@_hpsim with_dummy hpsim R RR) ps pt nths sti_src sti_tgt) fmr) 
+  | hpsim_intro (IN: hsupd (@_hpsim' with_dummy is_closed hpsim R RR (@_hpsim with_dummy is_closed hpsim R RR) ps pt nths sti_src sti_tgt) fmr) 
   .
 
-  Definition hpsim {R} RR := paco8 (@_hpsim false) bot8 R RR.
+  Definition hpsim is_closed {R} RR := paco8 (@_hpsim false is_closed) bot8 R RR.
+  (* Definition hpsim_closed {R} RR := paco8 (@_hpsim false true) bot8 R RR. *)
 
-  Lemma _hpsim_tarski with_dummy hpsim R RR rel
+  Lemma _hpsim_tarski with_dummy is_closed hpsim R RR rel
     (FIX: forall ps pt nths sti_src sti_tgt fmr
-            (IN: hsupd (@_hpsim' with_dummy hpsim R RR rel ps pt nths sti_src sti_tgt) fmr),
+            (IN: hsupd (@_hpsim' with_dummy is_closed hpsim R RR rel ps pt nths sti_src sti_tgt) fmr),
           rel ps pt nths sti_src sti_tgt fmr)
     :
-    @_hpsim with_dummy hpsim R RR <6= rel.
+    @_hpsim with_dummy is_closed hpsim R RR <6= rel.
   Proof.
     fix self 7. i.
     destruct PR. apply FIX.
@@ -291,29 +302,31 @@ Section HPSIM.
     des. esplits; eauto.
   Qed.
 
-  Lemma _hpsim'_mon with_dummy r r' R RR s s'
+  Lemma _hpsim'_mon with_dummy is_closed r r' R RR s s'
     ps pt nths sti_src sti_tgt fmr
-    (REL: @_hpsim' with_dummy r R RR s ps pt nths sti_src sti_tgt fmr)
+    (REL: @_hpsim' with_dummy is_closed r R RR s ps pt nths sti_src sti_tgt fmr)
     (LEr: r <8= r')
     (LEs: s <6= s')
     :
-    @_hpsim' with_dummy r' R RR s' ps pt nths sti_src sti_tgt fmr.
+    @_hpsim' with_dummy is_closed r' R RR s' ps pt nths sti_src sti_tgt fmr.
   Proof.
-    ii. destruct REL; des; esplits; eauto; econs; esplits; eauto.
+    ii. destruct REL; des; esplits; eauto.
+    24: { econs 24; eauto. }
+    all: econs; esplits; eauto.
   Qed.
   
-  Lemma _hpsim_mon with_dummy: monotone8 (@_hpsim with_dummy).
+  Lemma _hpsim_mon with_dummy is_closed : monotone8 (@_hpsim with_dummy is_closed).
   Proof.
     ii. eapply _hpsim_tarski, IN.
     i. econs. eauto using hsupd_mon, _hpsim'_mon.
   Qed.
 
-  Lemma _hpsim_mon_auto with_dummy r r' R RR
+  Lemma _hpsim_mon_auto with_dummy is_closed r r' R RR
     ps pt nths sti_src sti_tgt fmr
-    (REL: @_hpsim with_dummy r R RR ps pt nths sti_src sti_tgt fmr)
+    (REL: @_hpsim with_dummy is_closed r R RR ps pt nths sti_src sti_tgt fmr)
     (LEr: r <8= r')
     :
-    @_hpsim with_dummy r' R RR ps pt nths sti_src sti_tgt fmr.
+    @_hpsim with_dummy is_closed r' R RR ps pt nths sti_src sti_tgt fmr.
   Proof. eapply _hpsim_mon; eauto. Qed.
 
   Hint Constructors _hpsim' _hpsim.
@@ -325,18 +338,18 @@ Section HPSIM.
   Definition hpsim_tail : nat -> (alist key Any.t)*Any.t -> (alist key Any.t)*Any.t -> iProp :=
     fun nths '(st_src, v_src) '(st_tgt, v_tgt) => (⌜v_src = v_tgt⌝ ∗ Ist nths st_src st_tgt)%I.
 
-  Definition hpsim_body ps pt nths sti_src sti_tgt fmr :=
+  Definition hpsim_body is_closed ps pt nths sti_src sti_tgt fmr :=
     forall
       (NODFS: List.NoDup (List.map fst fl_src))
       (NODFT: List.NoDup (List.map fst fl_tgt))
       (NODS: List.NoDup (List.map fst sti_src.1))
       (NODD: List.NoDup (List.map fst sti_tgt.1)),
-    @hpsim _ hpsim_tail ps pt nths sti_src sti_tgt fmr.
+    @hpsim is_closed _ hpsim_tail ps pt nths sti_src sti_tgt fmr.
 
-  Definition hpsim_fun (i_src: itree hmodE Any.t) (i_tgt: itree hmodE Any.t):  Prop :=
+  Definition hpsim_fun is_closed (i_src: itree hmodE Any.t) (i_tgt: itree hmodE Any.t):  Prop :=
     forall nths st_src st_tgt fmr
            (INV: Own fmr ⊢ #=> Ist nths st_src st_tgt),
-      hpsim_body false false nths (st_src, i_src) (st_tgt, i_tgt) fmr.
+      hpsim_body is_closed false false nths (st_src, i_src) (st_tgt, i_tgt) fmr.
 
   Lemma case_itrH R (itrH: itree hmodE R) :
     (exists v, itrH = Ret v) \/
@@ -411,12 +424,12 @@ Section HPSIM.
     ii. eapply IN; eauto.
   Qed.  
 
-  Lemma _hpsim_flag_mon with_dummy r R RR (ps pt ps' pt': bool) nths st_src st_tgt fmr
-    (SIM: @_hpsim with_dummy r R RR ps pt nths st_src st_tgt fmr)
+  Lemma _hpsim_flag_mon with_dummy is_closed r R RR (ps pt ps' pt': bool) nths st_src st_tgt fmr
+    (SIM: @_hpsim with_dummy is_closed r R RR ps pt nths st_src st_tgt fmr)
     (LES: ps -> ps')
     (LET: pt -> pt')
     :
-    @_hpsim with_dummy r R RR ps' pt' nths st_src st_tgt fmr.
+    @_hpsim with_dummy is_closed r R RR ps' pt' nths st_src st_tgt fmr.
   Proof.
     move SIM before r. revert_until SIM.
     pattern ps, pt, nths, st_src, st_tgt, fmr.
@@ -428,39 +441,39 @@ Section HPSIM.
     econs; esplits; eauto.
   Qed.
 
-  Lemma hpsim_flag_mon R RR (ps pt ps' pt': bool) nths st_src st_tgt fmr
-    (SIM: @hpsim R RR ps pt nths st_src st_tgt fmr)
+  Lemma hpsim_flag_mon R RR is_closed (ps pt ps' pt': bool) nths st_src st_tgt fmr
+    (SIM: @hpsim is_closed R RR ps pt nths st_src st_tgt fmr)
     (LES: ps -> ps')
     (LET: pt -> pt')
     :
-    hpsim RR ps' pt' nths st_src st_tgt fmr.
+    hpsim is_closed RR ps' pt' nths st_src st_tgt fmr.
   Proof.
     move SIM before RR. revert_until SIM. pcofix CIH. i.
     pstep. eapply _hpsim_flag_mon; eauto.
     eapply paco8_mon_bot in SIM; eauto. punfold SIM.
   Qed.
 
-  Lemma hpsim_progress_flag with_dummy R RR r g nths st_src st_tgt fmr
-    (SIM: gpaco8 (@_hpsim with_dummy) (cpn8 (@_hpsim with_dummy)) g g R RR false false nths st_src st_tgt fmr)
+  Lemma hpsim_progress_flag with_dummy is_closed R RR r g nths st_src st_tgt fmr
+    (SIM: gpaco8 (@_hpsim with_dummy is_closed) (cpn8 (@_hpsim with_dummy is_closed)) g g R RR false false nths st_src st_tgt fmr)
     :
-    gpaco8 (@_hpsim with_dummy) (cpn8 (@_hpsim with_dummy)) r g R RR true true nths st_src st_tgt fmr.
+    gpaco8 (@_hpsim with_dummy is_closed) (cpn8 (@_hpsim with_dummy is_closed)) r g R RR true true nths st_src st_tgt fmr.
   Proof.
     gstep. econs. r; esplits; eauto.
   Qed.
 
 
   
-  Definition hpsimC with_dummy hpsim R RR ps pt nths sti_src sti_tgt fmr :=
-    hsupd (@_hpsim' with_dummy hpsim R RR (hpsim R RR) ps pt nths sti_src sti_tgt) fmr.
+  Definition hpsimC with_dummy is_closed hpsim R RR ps pt nths sti_src sti_tgt fmr :=
+    hsupd (@_hpsim' with_dummy is_closed hpsim R RR (hpsim R RR) ps pt nths sti_src sti_tgt) fmr.
   
-  Lemma hpsimC_mon with_dummy : monotone8 (@hpsimC with_dummy).
+  Lemma hpsimC_mon with_dummy is_closed : monotone8 (@hpsimC with_dummy is_closed).
   Proof.
     ii. specialize (IN H). des.
     destruct IN; econs; esplits; eauto; try by esplits; eauto.
   Qed.
 
-  Lemma hpsimC_spec with_dummy:
-    (@hpsimC with_dummy) <9= gupaco8 (@_hpsim with_dummy) (cpn8 (@_hpsim with_dummy)).
+  Lemma hpsimC_spec with_dummy is_closed:
+    (@hpsimC with_dummy is_closed) <9= gupaco8 (@_hpsim with_dummy is_closed) (cpn8 (@_hpsim with_dummy is_closed)).
   Proof.
     eapply wrespect8_uclo; eauto with paco.
     econs; eauto using hpsimC_mon; i.
@@ -484,18 +497,18 @@ Section HPSIM.
 
   Hint Resolve hpsim_flagC_mon: paco.
   
-  Lemma hpsim_flagC_spec with_dummy:
-    hpsim_flagC <9= gupaco8 (@_hpsim with_dummy) (cpn8 (@_hpsim with_dummy)).
+  Lemma hpsim_flagC_spec with_dummy is_closed:
+    hpsim_flagC <9= gupaco8 (@_hpsim with_dummy is_closed) (cpn8 (@_hpsim with_dummy is_closed)).
   Proof.
     eapply wrespect8_uclo; eauto with paco.
     econs; eauto with paco. i. inv PR.
     eauto using _hpsim_flag_mon, _hpsim_mon_auto, rclo8.
   Qed.
 
-  Lemma hpsim_flag_down with_dummy R RR r g ps pt nths st_src st_tgt fmr
-    (SIM: gpaco8 (@_hpsim with_dummy) (cpn8 (@_hpsim with_dummy)) r g R RR false false nths st_src st_tgt fmr)
+  Lemma hpsim_flag_down with_dummy is_closed R RR r g ps pt nths st_src st_tgt fmr
+    (SIM: gpaco8 (@_hpsim with_dummy is_closed) (cpn8 (@_hpsim with_dummy is_closed)) r g R RR false false nths st_src st_tgt fmr)
     :
-    gpaco8 (@_hpsim with_dummy) (cpn8 (@_hpsim with_dummy)) r g R RR ps pt nths st_src st_tgt fmr.
+    gpaco8 (@_hpsim with_dummy is_closed) (cpn8 (@_hpsim with_dummy is_closed)) r g R RR ps pt nths st_src st_tgt fmr.
   Proof. 
     guclo hpsim_flagC_spec. econs; et. 
   Qed.
@@ -526,8 +539,8 @@ Section HPSIM.
   .
   Proof. ii. destruct PR; econs; et. Qed.
 
-  Lemma hpsim_bindC_wrespectful with_dummy:
-    wrespectful8 (@_hpsim with_dummy) hpsim_bindC.
+  Lemma hpsim_bindC_wrespectful with_dummy is_closed:
+    wrespectful8 (@_hpsim with_dummy is_closed) hpsim_bindC.
   Proof.
     econs; eauto using hpsim_bindC_mon; i.
     destruct PR. apply GF in SIM.
@@ -544,24 +557,18 @@ Section HPSIM.
 
     exploit SIMK; eauto.
     i. apply GF in x0.
-    eapply (_hpsim_flag_mon _ _ _ _ _ _ ps0 pt0) in x0; try by i; clarify.
+    eapply (_hpsim_flag_mon _ _ _ _ _ _ _ ps0 pt0) in x0; try by i; clarify.
 
     destruct x0. eapply hsupd_update in IN; eauto.
     eapply _hpsim_mon_auto; eauto using rclo8.
   Qed.
 
-  Lemma hpsim_bindC_spec with_dummy:
-    hpsim_bindC <9= gupaco8 (@_hpsim with_dummy) (cpn8 (@_hpsim with_dummy)).
+  Lemma hpsim_bindC_spec with_dummy is_closed:
+    hpsim_bindC <9= gupaco8 (@_hpsim with_dummy is_closed) (cpn8 (@_hpsim with_dummy is_closed)).
   Proof.
     intros. eapply wrespect8_uclo; eauto with paco.
     apply hpsim_bindC_wrespectful.
   Qed.
-
-
-
-
-
-
 
   Variant hpsim_extendC (r: forall R (RR: nat -> (alist key Any.t) * R -> (alist key Any.t) * R -> iProp), bool -> bool -> nat -> (alist key Any.t) * itree hmodE R -> (alist key Any.t) * itree hmodE R -> Σ -> Prop):
     forall R (RR: nat -> (alist key Any.t) * R -> (alist key Any.t) * R -> iProp), bool -> bool -> nat -> (alist key Any.t) * itree hmodE R -> (alist key Any.t) * itree hmodE R -> Σ -> Prop
@@ -582,8 +589,8 @@ Section HPSIM.
   .
   Proof. ii. destruct PR; econs; et. Qed.
 
-  Lemma hpsim_extendC_compatible with_dummy:
-    compatible8 (@_hpsim with_dummy) hpsim_extendC.
+  Lemma hpsim_extendC_compatible with_dummy is_closed:
+    compatible8 (@_hpsim with_dummy is_closed) hpsim_extendC.
   Proof.
     econs; eauto using hpsim_extendC_mon.
     intros. destruct PR. destruct SIM. econs.
@@ -592,8 +599,8 @@ Section HPSIM.
     i. econs; eauto; refl.
   Qed.
   
-  Lemma hpsim_extendC_spec with_dummy:
-    hpsim_extendC <9= gupaco8 (@_hpsim with_dummy) (cpn8 (@_hpsim with_dummy)).
+  Lemma hpsim_extendC_spec with_dummy is_closed:
+    hpsim_extendC <9= gupaco8 (@_hpsim with_dummy is_closed) (cpn8 (@_hpsim with_dummy is_closed)).
   Proof.
     intros. gclo. econs; eauto using hpsim_extendC_compatible.
     eapply hpsim_extendC_mon, PR; eauto with paco.
@@ -624,16 +631,16 @@ Section HPSIM.
     ii. destruct PR. econs; eauto using hsupd_mon.
   Qed.
 
-  Lemma hpsim_wfC_compatible with_dummy:
-    compatible8 (@_hpsim with_dummy) hpsim_wfC.
+  Lemma hpsim_wfC_compatible with_dummy is_closed:
+    compatible8 (@_hpsim with_dummy is_closed) hpsim_wfC.
   Proof.
     econs; eauto using hpsim_wfC_mon.
     i. destruct PR. econs. eapply hsupd_wf. i.
     eapply _hpsim_mon_auto; eauto 10 using hpsim_wfC, hsupd_incl with paco.
   Qed.
   
-  Lemma hpsim_wfC_spec with_dummy:
-    hpsim_wfC <9= gupaco8 (@_hpsim with_dummy) (cpn8 (@_hpsim with_dummy)).
+  Lemma hpsim_wfC_spec with_dummy is_closed:
+    hpsim_wfC <9= gupaco8 (@_hpsim with_dummy is_closed) (cpn8 (@_hpsim with_dummy is_closed)).
   Proof.
     intros. gclo. econs; eauto using hpsim_wfC_compatible.
     eapply hpsim_wfC_mon, PR; eauto with paco.
@@ -663,8 +670,8 @@ Section HPSIM.
     ii. destruct PR. econs; eauto using hsupd_mon.
   Qed.
 
-  Lemma hpsim_updateC_compatible with_dummy:
-    compatible8 (@_hpsim with_dummy) hpsim_updateC.
+  Lemma hpsim_updateC_compatible with_dummy is_closed:
+    compatible8 (@_hpsim with_dummy is_closed) hpsim_updateC.
   Proof.
     econs; eauto using hpsim_updateC_mon.
     i. destruct PR. econs. eapply hsupd_merge.
@@ -673,9 +680,9 @@ Section HPSIM.
     eauto 10 using hpsim_updateC, hsupd_incl with paco.
   Qed.
   
-  Lemma hpsim_updateC_spec with_dummy:
-    hpsim_updateC <9= gupaco8 (@_hpsim with_dummy) (cpn8 (@_hpsim with_dummy)).
-  Proof.
+  Lemma hpsim_updateC_spec with_dummy is_closed:
+    hpsim_updateC <9= gupaco8 (@_hpsim with_dummy is_closed) (cpn8 (@_hpsim with_dummy is_closed)).
+  Proof. 
     intros. gclo. econs; eauto using hpsim_updateC_compatible.
     eapply hpsim_updateC_mon, PR; eauto with paco.
   Qed.
@@ -703,8 +710,8 @@ Section HPSIM.
     ii. destruct PR. econs; eauto using hsupd_mon.
   Qed.
   
-  Lemma hpsim_frameC_compatible with_dummy:
-    compatible8 (@_hpsim with_dummy) hpsim_frameC.
+  Lemma hpsim_frameC_compatible with_dummy is_closed:
+    compatible8 (@_hpsim with_dummy is_closed) hpsim_frameC.
   Proof.
     econs; eauto using hpsim_frameC_mon. i.
     destruct PR. move SIM before r. revert_until SIM.
@@ -826,20 +833,19 @@ Section HPSIM.
     - eauto using hpsim_frameC with paco.
   Qed.
   
-  Lemma hpsim_frameC_spec with_dummy:
-    hpsim_frameC <9= gupaco8 (@_hpsim with_dummy) (cpn8 (@_hpsim with_dummy)).
+  Lemma hpsim_frameC_spec with_dummy is_closed:
+    hpsim_frameC <9= gupaco8 (@_hpsim with_dummy is_closed) (cpn8 (@_hpsim with_dummy is_closed)).
   Proof.
     intros. gclo. econs; eauto using hpsim_frameC_compatible.
     eapply hpsim_frameC_mon, PR; eauto with paco.
   Qed.
 
-  
-
-  Definition hpsim_fsem: relation (Any.t -> itree hmodE Any.t) :=
+  (* not used in anywhere *)
+  (* Definition hpsim_fsem: relation (Any.t -> itree hmodE Any.t) :=
     (eq ==> hpsim_fun)%signature.
   
   Definition hpsim_fnsem: relation (string * (Any.t -> itree hmodE Any.t)) :=
-    RelProd eq hpsim_fsem.
+    RelProd eq hpsim_fsem. *)
   
 End HPSIM.
 
