simulations/isim/ISim.v
@@ -29,16 +29,16 @@ Section LEMMAS.
 (***** Move and rename: HoareCall LEMMAS *****)
 
   Lemma hcall_clo Σ
-    fls flt I my_tid r g ps pt {R} RR nths st_src st_tgt k_src k_tgt
+    fls flt I my_tid is_closed r g ps pt {R} RR nths st_src st_tgt k_src k_tgt
     fn varg arg X (x: shelve__ X) P Q
   :
     (P my_tid x varg arg 
       ∗ I nths st_src st_tgt 
       ∗ (∀ nths0 st_src0 st_tgt0 vret ret, 
              (Q my_tid x vret ret ∗ I nths0 st_src0 st_tgt0) 
-          -∗ @isim Σ fls flt I my_tid r g R RR true true nths0 (st_src0, k_src vret) (st_tgt0, k_tgt ret)))
+          -∗ @isim Σ fls flt I my_tid is_closed r g R RR true true nths0 (st_src0, k_src vret) (st_tgt0, k_tgt ret)))
   -∗  
-    @isim _ fls flt I my_tid r g R RR ps pt nths (st_src, HoareCall (mk_fspec P Q) fn varg >>= k_src) (st_tgt, trigger (Call fn arg) >>= k_tgt).
+    @isim _ fls flt I my_tid is_closed r g R RR ps pt nths (st_src, HoareCall (mk_fspec P Q) fn varg >>= k_src) (st_tgt, trigger (Call fn arg) >>= k_tgt).
   Proof.
     iIntros "(P & IST & K)".
     unfold HoareCall. prep. steps_l.
@@ -86,7 +86,7 @@ Section HModProd.
     rewrite /state_scopes -!List.map_map alist_upd_keys. eauto.
   Qed.
   
-  Lemma isim_reflR Ist fl_src fl_tgt scopesL scopesR scopesF (EqR: _->_->_->iProp) itr
+  Lemma isim_reflR Ist is_closed fl_src fl_tgt scopesL scopesR scopesF (EqR: _->_->_->iProp) itr
     (DISJ: List.NoDup (scopesL ++ scopesR))
     (INCL: incl scopesF scopesR)
     (EQGET: ∀ nths st_src st_tgt,
@@ -95,7 +95,7 @@ Section HModProd.
         EqR nths st_src st_tgt -∗
           EqR nths0 (alist_upd k v st_src) (alist_upd k v st_tgt))
     :
-    isim_fsem fl_src fl_tgt (IstProd0 (IstSB0 scopesL Ist) EqR)
+    isim_fsem fl_src fl_tgt (IstProd0 (IstSB0 scopesL Ist) EqR) is_closed
       (HModSem.sandbox_body (scopesF,itr)) (HModSem.sandbox_body (scopesF,itr)).
   Proof.
     ii. subst. unfold HModSem.sandbox_body. s.
@@ -165,7 +165,7 @@ Section HModProd.
   { eapply alist_upd_nodup. eauto. }
   Qed.
 
-  Lemma mod_sim_reflR A B C init_cond Ist
+  Lemma mod_sim_reflR A B C init_cond Ist is_closed
     (INIT: ∀ sk, init_cond sk -∗
                     IstProd (IstSB A Ist) IstEq sk 1
                     (HModSem.initial_st (HMod.modsem (HMod.add A C) sk))
@@ -180,11 +180,11 @@ Section HModProd.
            In fn (List.map fst (HModSem.fnsems (HMod.modsem B sk))))
     (SIM: ∀ sk fn
             (IN: In fn (List.map fst (HModSem.fnsems (HMod.modsem A sk)))),
-          HSSim.sim_fun (HMod.modsem (HMod.add A C) sk) (HMod.modsem (HMod.add B C) sk)
+          HSSim.sim_fun is_closed (HMod.modsem (HMod.add A C) sk) (HMod.modsem (HMod.add B C) sk)
             (IstProd (IstSB A Ist) IstEq sk) fn)
     (SK: HMod.sk A = HMod.sk B)
     :
-    HSim.t (HMod.add A C) (HMod.add B C) init_cond (IstProd (IstSB A Ist) IstEq).
+    HSim.t is_closed (HMod.add A C) (HMod.add B C) init_cond (IstProd (IstSB A Ist) IstEq).
   Proof.
     econs; cycle 1.
     { rr. eapply Permutation_app_tail. rewrite SK. refl. }
