simulations/isim/ITacticsCore.v
@@ -324,26 +324,26 @@ Ltac _step_l :=
   match goal with
   (******* isim ******)
   (** src **)
-  | [ |- environments.envs_entails _ (isim _ _ _ _ _ _ _ _ _ _ (_, tau;; _) _) ] =>
+  | [ |- environments.envs_entails _ (isim _ _ _ _ _ _ _ _ _ _ _ (_, tau;; _) _) ] =>
       iApply isim_tau_src
-  | [ |- environments.envs_entails _ (isim _ _ _ _ _ _ _ _ _ _ (_, Ret _ >>= _) _) ] =>
+  | [ |- environments.envs_entails _ (isim _ _ _ _ _ _ _ _ _ _ _ (_, Ret _ >>= _) _) ] =>
       rewrite bind_ret_l
-  | [ |- environments.envs_entails _ (isim _ _ _ _ _ _ _ _ _ _ (_, (HModSem.sandbox _ (trigger (SPut _ _))) >>= _) _) ] =>
+  | [ |- environments.envs_entails _ (isim _ _ _ _ _ _ _ _ _ _ _ (_, (HModSem.sandbox _ (trigger (SPut _ _))) >>= _) _) ] =>
       iApply isim_sput_src_sandbox; [s;eauto|]
-  | [ |- environments.envs_entails _ (isim _ _ _ _ _ _ _ _ _ _ (_, (HModSem.sandbox _ (trigger (SGet _))) >>= _) _) ] =>
+  | [ |- environments.envs_entails _ (isim _ _ _ _ _ _ _ _ _ _ _ (_, (HModSem.sandbox _ (trigger (SGet _))) >>= _) _) ] =>
       iApply isim_sget_src_sandbox; [s;eauto|]
-  | [ |- environments.envs_entails _ (isim _ _ _ _ _ _ _ _ _ _ (_, trigger (Take _) >>= _) _) ] =>
+  | [ |- environments.envs_entails _ (isim _ _ _ _ _ _ _ _ _ _ _ (_, trigger (Take _) >>= _) _) ] =>
       let name := fresh "q" in
       iApply isim_take_src; iIntros (name)
-  | [ |- environments.envs_entails _ (isim _ _ _ _ _ _ _ _ _ _  (_, trigger (Assume ?P) >>= _) _) ] =>
+  | [ |- environments.envs_entails _ (isim _ _ _ _ _ _ _ _ _ _ _  (_, trigger (Assume ?P) >>= _) _) ] =>
       unfold_precond_postcond P; iApply isim_Assume_src; iIntrosFresh "ASM"
-  | [ |- environments.envs_entails _ (isim _ _ _ _ _ _ _ _ _ _ (_, unwrapU ?ox >>= _) _) ] =>
+  | [ |- environments.envs_entails _ (isim _ _ _ _ _ _ _ _ _ _ _ (_, unwrapU ?ox >>= _) _) ] =>
       let name := fresh "q" in
       iApply isim_unwrapU_src; iIntros (name) "%";
       match goal with [ H: ?x = Some _ |- _ ] => let G := fresh "G" in rename H into G; try rewrite G in * end
-  | [ |- environments.envs_entails _ (isim _ _ _ _ _ _ _ _ _ _ (_, assume _ >>= _) _) ] =>
+  | [ |- environments.envs_entails _ (isim _ _ _ _ _ _ _ _ _ _ _ (_, assume _ >>= _) _) ] =>
       let name := fresh "asm" in iApply isim_asm_src; iIntros (name)
-  | [ |- environments.envs_entails _ (isim _ _ _ _ _ _ _ _ _ _ (_, trigger Tid >>= _) _) ] =>
+  | [ |- environments.envs_entails _ (isim _ _ _ _ _ _ _ _ _ _ _ (_, trigger Tid >>= _) _) ] =>
       iApply isim_tid_src
   end.
 
@@ -351,26 +351,26 @@ Ltac _step_r :=
   match goal with
   (******* isim ******)
   (** tgt **)
-  | [ |- environments.envs_entails _ (isim _ _ _ _ _ _ _ _ _ _ _ (_, Ret _ >>= _)) ] =>
+  | [ |- environments.envs_entails _ (isim _ _ _ _ _ _ _ _ _ _ _ _ (_, Ret _ >>= _)) ] =>
       rewrite bind_ret_l
-  | [ |- environments.envs_entails _ (isim _ _ _ _ _ _ _ _ _ _ _ (_, tau;; _)) ] =>
+  | [ |- environments.envs_entails _ (isim _ _ _ _ _ _ _ _ _ _ _ _ (_, tau;; _)) ] =>
       iApply isim_tau_tgt
-  | [ |- environments.envs_entails _ (isim _ _ _ _ _ _ _ _ _ _ _ (_, (HModSem.sandbox _ (trigger (SPut _ _))) >>= _)) ] =>
+  | [ |- environments.envs_entails _ (isim _ _ _ _ _ _ _ _ _ _ _ _ (_, (HModSem.sandbox _ (trigger (SPut _ _))) >>= _)) ] =>
       iApply isim_sput_tgt_sandbox; [s; eauto|]
-  | [ |- environments.envs_entails _ (isim _ _ _ _ _ _ _ _ _ _ _ (_, (HModSem.sandbox _ (trigger (SGet _))) >>= _)) ] =>
+  | [ |- environments.envs_entails _ (isim _ _ _ _ _ _ _ _ _ _ _ _ (_, (HModSem.sandbox _ (trigger (SGet _))) >>= _)) ] =>
       iApply isim_sget_tgt_sandbox; [s; eauto|]
-  | [ |- environments.envs_entails _ (isim _ _ _ _ _ _ _ _ _ _ _ (_, trigger (Choose _) >>= _)) ] =>
+  | [ |- environments.envs_entails _ (isim _ _ _ _ _ _ _ _ _ _ _ _ (_, trigger (Choose _) >>= _)) ] =>
       let name := fresh "q" in
       iApply isim_choose_tgt; iIntros (name)
-  | [ |- environments.envs_entails _ (isim _ _ _ _ _ _ _ _ _ _ _ (_, trigger (Guarantee ?P) >>= _)) ] =>
+  | [ |- environments.envs_entails _ (isim _ _ _ _ _ _ _ _ _ _ _ _ (_, trigger (Guarantee ?P) >>= _)) ] =>
       unfold_precond_postcond P; iApply isim_Guarantee_tgt; iIntrosFresh "GRT"
-  | [ |- environments.envs_entails _ (isim _ _ _ _ _ _ _ _ _ _ _ (_, unwrapN ?ox >>= _)) ] =>
+  | [ |- environments.envs_entails _ (isim _ _ _ _ _ _ _ _ _ _ _ _ (_, unwrapN ?ox >>= _)) ] =>
       let name := fresh "q" in
       iApply isim_unwrapN_tgt; iIntros (name) "%";
       match goal with [ H: ?x = Some _ |- _ ] => let G := fresh "G" in rename H into G; try rewrite G in * end
-  | [ |- environments.envs_entails _ (isim _ _ _ _ _ _ _ _ _ _ _ (_, guarantee _ >>= _)) ] =>
+  | [ |- environments.envs_entails _ (isim _ _ _ _ _ _ _ _ _ _ _ _ (_, guarantee _ >>= _)) ] =>
       let name := fresh "grt" in iApply isim_guar_tgt; iIntros (name)
-  | [ |- environments.envs_entails _ (isim _ _ _ _ _ _ _ _ _ _ _ (_, trigger Tid >>=  _)) ] =>
+  | [ |- environments.envs_entails _ (isim _ _ _ _ _ _ _ _ _ _ _ _ (_, trigger Tid >>=  _)) ] =>
       iApply isim_tid_tgt
   end.
 
@@ -378,36 +378,36 @@ Ltac _step :=
   match goal with
   (******* isim ******)
   (** both **)
-  | [ |- environments.envs_entails _ (isim _ _ _ _ _ _ _ _ _ _ (_, Ret _) (_, Ret _)) ] =>
+  | [ |- environments.envs_entails _ (isim _ _ _ _ _ _ _ _ _ _ _ (_, Ret _) (_, Ret _)) ] =>
       iApply isim_ret
-  | [ |- environments.envs_entails _ (isim _ _ _ _ _ _ _ _ _ _ (_, trigger (IO _ _) >>= _) (_, trigger (IO _ _) >>= _)) ] =>
+  | [ |- environments.envs_entails _ (isim _ _ _ _ _ _ _ _ _ _ _ (_, trigger (IO _ _) >>= _) (_, trigger (IO _ _) >>= _)) ] =>
       iApply isim_io; iIntros "%"
-  | [ |- environments.envs_entails _ (isim _ _ _ _ _ _ _ _ _ _ (_, trigger (Spawn _ _) >>= _) (_, trigger (Spawn _ _) >>= _)) ] =>
+  | [ |- environments.envs_entails _ (isim _ _ _ _ _ _ _ _ _ _ _ (_, trigger (Spawn _ _) >>= _) (_, trigger (Spawn _ _) >>= _)) ] =>
       iApply isim_spawn
   end.
 
 Ltac _force_l :=
   match goal with
-  | [ |- environments.envs_entails _ (isim _ _ _ _ _ _ _ _ _ _ (_, trigger (Choose ?T) >>= _) _) ] =>
+  | [ |- environments.envs_entails _ (isim _ _ _ _ _ _ _ _ _ _ _ (_, trigger (Choose ?T) >>= _) _) ] =>
       iApply isim_choose_src
-  | [ |- environments.envs_entails _ (isim _ _ _ _ _ _ _ _ _ _ (_, trigger (Guarantee ?P) >>= _) _) ] =>
+  | [ |- environments.envs_entails _ (isim _ _ _ _ _ _ _ _ _ _ _ (_, trigger (Guarantee ?P) >>= _) _) ] =>
       unfold_precond_postcond P; iApply isim_Guarantee_src
-  | [ |- environments.envs_entails _ (isim _ _ _ _ _ _ _ _ _ _ (_, unwrapN _ >>= _) _) ] =>
+  | [ |- environments.envs_entails _ (isim _ _ _ _ _ _ _ _ _ _ _ (_, unwrapN _ >>= _) _) ] =>
       iApply isim_unwrapN_src; iExists _
-  | [ |- environments.envs_entails _ (isim _ _ _ _ _ _ _ _ _ _ (_, guarantee _ >>= _) _) ] =>
+  | [ |- environments.envs_entails _ (isim _ _ _ _ _ _ _ _ _ _ _ (_, guarantee _ >>= _) _) ] =>
       iApply isim_guar_src
   end
 .
 
 Ltac _force_r :=
   match goal with
-  | [ |- environments.envs_entails _ (isim _ _ _ _ _ _ _ _ _ _ _ (_, trigger (Take _) >>= _)) ] =>
+  | [ |- environments.envs_entails _ (isim _ _ _ _ _ _ _ _ _ _ _ _ (_, trigger (Take _) >>= _)) ] =>
       iApply isim_take_tgt
-  | [ |- environments.envs_entails _ (isim _ _ _ _ _ _ _ _ _ _ _ (_, trigger (Assume ?P) >>= _)) ] =>
+  | [ |- environments.envs_entails _ (isim _ _ _ _ _ _ _ _ _ _ _ _ (_, trigger (Assume ?P) >>= _)) ] =>
       unfold_precond_postcond P; iApply isim_Assume_tgt
-  | [ |- environments.envs_entails _ (isim _ _ _ _ _ _ _ _ _ _ _ (_, unwrapU _ >>= _)) ] =>
+  | [ |- environments.envs_entails _ (isim _ _ _ _ _ _ _ _ _ _ _ _ (_, unwrapU _ >>= _)) ] =>
       iApply isim_unwrapU_tgt; iExists _
-  | [ |- environments.envs_entails _ (isim _ _ _ _ _ _ _ _ _ _ _ (_, assume _ >>= _)) ] =>
+  | [ |- environments.envs_entails _ (isim _ _ _ _ _ _ _ _ _ _ _ _ (_, assume _ >>= _)) ] =>
       iApply isim_asm_tgt
   end
 .
@@ -602,37 +602,37 @@ Local Notation level := nat.
 (*** isim ***)
 Notation "E1 '------------------------------------------------------------------□' E2 '------------------------------------------------------------------∗' st_src st_tgt '-------------------------------isim-------------------------------'  itr_src itr_tgt"
 :=
-  (environments.envs_entails (Envs E1 E2 _) (isim _ _ _ _ _ _ _ _ _ _ (st_src, itr_src) (st_tgt, itr_tgt)))
+  (environments.envs_entails (Envs E1 E2 _) (isim _ _ _ _ _ _ _ _ _ _ _ (st_src, itr_src) (st_tgt, itr_tgt)))
     (at level 50,
      format "E1 '------------------------------------------------------------------□' '//' E2 '------------------------------------------------------------------∗' '//' st_src '//' st_tgt '//' '-------------------------------isim-------------------------------' '//' itr_src '//' '//' '//' itr_tgt '//' ").
 
 Notation "E1 '------------------------------------------------------------------□' st_src st_tgt '-------------------------------isim-------------------------------'  itr_src itr_tgt"
 :=
-  (environments.envs_entails (Envs E1 Enil _) (isim _ _ _ _ _ _ _ _ _ _ (st_src, itr_src) (st_tgt, itr_tgt)))
+  (environments.envs_entails (Envs E1 Enil _) (isim _ _ _ _ _ _ _ _ _ _ _ (st_src, itr_src) (st_tgt, itr_tgt)))
     (at level 50,
      format "E1 '------------------------------------------------------------------□' '//' st_src '//' st_tgt '//' '-------------------------------isim-------------------------------' '//' itr_src '//' '//' '//' itr_tgt '//' ").
 
 Notation "E2 '------------------------------------------------------------------∗' st_src st_tgt '-------------------------------isim-------------------------------'  itr_src itr_tgt"
 :=
-  (environments.envs_entails (Envs Enil E2 _) (isim _ _ _ _ _ _ _ _ _ _ (st_src, itr_src) (st_tgt, itr_tgt)))
+  (environments.envs_entails (Envs Enil E2 _) (isim _ _ _ _ _ _ _ _ _ _ _ (st_src, itr_src) (st_tgt, itr_tgt)))
     (at level 50,
      format "E2 '------------------------------------------------------------------∗' '//' st_src '//' st_tgt '//' '-------------------------------isim-------------------------------' '//' itr_src '//' '//' '//' itr_tgt '//' ").
 
 Notation "'------------------------------------------------------------------∗' st_src st_tgt '-------------------------------isim-------------------------------'  itr_src itr_tgt"
 :=
-  (environments.envs_entails (Envs Enil Enil _) (isim _ _ _ _ _ _ _ _ _ _ (st_src, itr_src) (st_tgt, itr_tgt)))
+  (environments.envs_entails (Envs Enil Enil _) (isim _ _ _ _ _ _ _ _ _ _ _ (st_src, itr_src) (st_tgt, itr_tgt)))
     (at level 50,
      format "'------------------------------------------------------------------∗' '//' st_src '//' st_tgt '//' '-------------------------------isim-------------------------------' '//' itr_src '//' '//' '//' itr_tgt '//' ").
 
 (* additional *) 
 Notation "E1 '------------------------------------------------------------------□' E2 '------------------------------------------------------------------∗' st_src st_tgt '-------------------------------isim-------------------------------'  P '∗' 'ISIM'"
 :=
-  (environments.envs_entails (Envs E1 E2 _) (bi_sep P (isim _ _ _ _ _ _ _ _ _ _ (st_src, _) (st_tgt, _))))
+  (environments.envs_entails (Envs E1 E2 _) (bi_sep P (isim _ _ _ _ _ _ _ _ _ _ _ (st_src, _) (st_tgt, _))))
     (at level 50,
      format "E1 '------------------------------------------------------------------□' '//' E2 '------------------------------------------------------------------∗' '//' st_src '//' st_tgt '//' '-------------------------------isim-------------------------------' '//' P  '∗'  'ISIM' ").
 
 Notation "E1 '------------------------------------------------------------------□' E2 '------------------------------------------------------------------∗' st_src st_tgt '-------------------------------isim-------------------------------'  P '-∗' 'ISIM'"
 :=
-  (environments.envs_entails (Envs E1 E2 _) (bi_wand P (isim _ _ _ _ _ _ _ _ _ _ (st_src, _) (st_tgt, _))))
+  (environments.envs_entails (Envs E1 E2 _) (bi_wand P (isim _ _ _ _ _ _ _ _ _ _ _ (st_src, _) (st_tgt, _))))
     (at level 50,
      format "E1 '------------------------------------------------------------------□' '//' E2 '------------------------------------------------------------------∗' '//' st_src '//' st_tgt '//' '-------------------------------isim-------------------------------' '//' P  '-∗'  'ISIM' ").
