simulations/modsim/ModSim.v
@@ -199,6 +199,16 @@ Section SIM_ITREE.
     sim_itree_def sim_itree RR self ps pt w nths (st_src, i_src)
       (st_tgt, trigger Tid >>= k_tgt)
       
+  | sim_itree_call_none
+      ps pt w nths st_src st_tgt
+      fn varg i_src k_tgt
+      (FUN: alist_find fn fl_tgt = None)
+      (K: self ps true w nths (st_src, i_src) (st_tgt, triggerNB >>= k_tgt))
+    :
+    sim_itree_def sim_itree RR self ps pt w nths
+      (st_src, i_src)
+      (st_tgt, trigger (Call fn varg) >>= k_tgt)
+
   | sim_itree_progress
       w w0 nths st_src st_tgt 
       i_src i_tgt
@@ -241,7 +251,9 @@ Section SIM_ITREE.
   Lemma sim_itree_mon: monotone9 _sim_itree.
   Proof.
     ii. eapply sim_itree_tarski; eauto.
-    econs; inv PR; econs; eauto.
+    econs; inv PR. 
+    18: { econs 18; eauto. }
+    all: econs; eauto.
   Qed.
 
   Hint Constructors _sim_itree.
@@ -343,6 +355,7 @@ Section SIM_ITREE.
     { econs 15; eauto. des. esplits; eauto. eapply sim_itree_mon; eauto. i. eapply rclo9_base. eauto.  }
     { econs 16; eauto. des. esplits; eauto. eapply sim_itree_mon; eauto. i. eapply rclo9_base. eauto.  }
     { econs 17; eauto. des. esplits; eauto. eapply sim_itree_mon; eauto. i. eapply rclo9_base. eauto.  }
+    { econs 18; eauto. des. esplits; eauto. eapply sim_itree_mon; eauto. i. eapply rclo9_base. eauto.  }
     { ss. }
   Qed.
 
@@ -370,7 +383,8 @@ Section SIM_ITREE.
     { guclo sim_itree_indC_spec. econs 15; eauto. gbase. eauto. }
     { guclo sim_itree_indC_spec. econs 16; eauto. gbase. eauto. }
     { guclo sim_itree_indC_spec. econs 17; eauto. gbase. eauto. }
-    { guclo sim_itree_indC_spec. econs 18; eauto. }
+    { guclo sim_itree_indC_spec. econs 18; eauto. gbase. eauto. }
+    { guclo sim_itree_indC_spec. econs 19; eauto. }
   Qed.
 
   Lemma sim_itreeC_spec r g
@@ -475,7 +489,9 @@ Section SIM_ITREE.
     gcofix CIH. 
     i. revert ps pt. pattern b, b0, w, nths, st_src, st_tgt.
     eapply sim_itree_ind, SIM. i.
-    inv PR; ss; i; clarify; try (guclo sim_itree_indC_spec; hdes; econs; eauto).
+    inv PR; ss; i; clarify.
+    18: { guclo sim_itree_indC_spec. hdes. econs 18; eauto. }
+    all: try (guclo sim_itree_indC_spec; hdes; econs; eauto).
     eapply sim_itree_flag_down. gfinal. right.
     eapply paco9_mon.
     - punfold SIM0. pstep. eapply sim_itree_wmon; eauto using le_others_refl.
@@ -517,7 +533,11 @@ Section SIM_ITREE.
     move SIM before GF. revert_until SIM. eapply GF in SIM.
     pattern x3, x4, x5, x6, p, p0.
     eapply sim_itree_tarski, SIM.
-    i. inv PR; clarify; grind; try (econs; econs; eauto).
+    i. inv PR; clarify; grind; try econs. 
+    18: { econs 18; eauto. exploit K; et. i.  
+          rewrite !bind_bind in *. eauto.
+    }
+    all: try (econs; eauto).
     - exploit SIMK; eauto. i.
       eapply sim_itree_flag_mon with (ps0 := false) (pt0 := false); ss.
       eapply sim_itree_mon.
